signature to spec

code/experimental/P256/Hacl.Impl.ECDSA.P256SHA256.Signature.fst
@@ -240,7 +240,6 @@ val ecdsa_signature_nist_compliant: result: lbuffer uint8 (size 64) -> m: lbuffe
       let resultR = nat_from_bytes_le (as_seq h1 resultR) in 
       let resultS = nat_from_bytes_le (as_seq h1 resultS) in 
       flag == flagSpec /\ r == resultR /\ s == resultS
-   
     )
   )
 
@@ -274,6 +273,7 @@ val ecdsa_signature_core: r: felem -> s: felem -> mLen: size_t -> m: lbuffer uin
     live h r /\ live h s /\ live h m /\ live h privKeyAsFelem /\ live h k /\
     disjoint privKeyAsFelem r /\ disjoint k r /\ disjoint r s /\
     as_nat h privKeyAsFelem < prime_p256_order /\
+    as_nat h s == 0 /\
     nat_from_bytes_le (as_seq h k) < prime_p256_order
   )
   (ensures fun h0 flag h1 -> 
@@ -290,7 +290,7 @@ val ecdsa_signature_core: r: felem -> s: felem -> mLen: size_t -> m: lbuffer uin
       let kFelem = nat_from_bytes_le (as_seq h0 k) in 
       as_nat h1 r == xN % prime_p256_order /\
       (
-	if as_nat h1 r = 0 then flag = false else
+	if as_nat h1 r = 0 then begin flag = false /\ as_nat h1 s == 0 end else
 	  as_nat h1 s == (z + (as_nat h1 r) * as_nat h0 privKeyAsFelem) * pow kFelem (prime_p256_order - 2) % prime_p256_order /\
 	  (
 	    if (as_nat h1 s = 0) then flag = false else flag = true
@@ -338,32 +338,13 @@ val ecdsa_signature: result: lbuffer uint8 (size 64) -> mLen: size_t -> m: lbuff
   )
   (ensures fun h0 flag h1 -> 
     modifies (loc result) h0 h1 /\
-    (
+     (
       let resultR = gsub result (size 0) (size 32) in 
       let resultS = gsub result (size 32) (size 32) in 
-
-      let hashM = Spec.Hash.hash Spec.Hash.Definitions.SHA2_256 (as_seq h0 m) in 
-      let hashChanged = Hacl.Spec.ECDSA.changeEndian (uints_from_bytes_be hashM) in
-      let z = nat_from_intseq_le hashChanged % prime_p256_order in 
-
-      let basePoint = (0x6B17D1F2E12C4247F8BCE6E563A440F277037D812DEB33A0F4A13945D898C296, 0x4FE342E2FE1A7F9B8EE7EB4A7C0F9E162BCE33576B315ECECBB6406837BF51F5, 1) in
-      let (rxN, ryN, rzN), _ = montgomery_ladder_spec (as_seq h0 k) ((0,0,0), basePoint) in 
-      let (xN, _, _) = _norm (rxN, ryN, rzN) in 
-      
-      let kFelem = nat_from_bytes_le (as_seq h0 k) in 
-      let privateKey = nat_from_bytes_le (as_seq h0 privKey) in 
-
+      let r, s, flagSpec = Hacl.Spec.ECDSA.ecdsa_signature (uint_v mLen) (as_seq h0 m) (as_seq h0 privKey) (as_seq h0 k) in 
       let resultR = nat_from_bytes_le (as_seq h1 resultR) in 
       let resultS = nat_from_bytes_le (as_seq h1 resultS) in 
-
-      resultR == xN % prime_p256_order /\
-      (
-	if resultR = 0 then flag = false else
-	  resultS == (z + resultR * privateKey) * pow kFelem (prime_p256_order - 2) % prime_p256_order /\
-	  (
-	    if (resultS = 0) then flag = false else flag = true
-	  )
-      )
+      flag == flagSpec /\ r == resultR /\ s == resultS
     )    
   )
 
